intermediate/Veritas.Intermediate.Correctness.fst
@@ -5,15 +5,20 @@ open Veritas.Record
 open Veritas.SeqMachine
 open Veritas.State
 open Veritas.StateSeqMachine
+open Veritas.Verifier
 open Veritas.Verifier.EAC
 open Veritas.Intermediate.Global
+open Veritas.Intermediate.Logs
 open Veritas.Intermediate.Thread
 open Veritas.Intermediate.TSLog
+open Veritas.Intermediate.Verify
 open Veritas.Intermediate.VerifierConfig
 
 module I = Veritas.Interleave
 module IntL = Veritas.Intermediate.Logs
 module IntG = Veritas.Intermediate.Global
+module IntV = Veritas.Intermediate.Verify
+module IntS = Veritas.Intermediate.Store
 module IntTS = Veritas.Intermediate.TSLog
 module SpecTS = Veritas.Verifier.TSLog
 module SpecC = Veritas.Verifier.Correctness
@@ -34,6 +39,75 @@ let induction_props #vcfg (ils: its_log vcfg) =
 let induction_props_or_hash_collision #vcfg (ils: its_log vcfg) = 
   o:option hash_collision_gen{Some? o \/ induction_props ils}
 
+
+let lemma_eac_boundary_inv (itsl: SpecTS.its_log) (i:I.seq_index itsl): 
+  Lemma (requires (SpecTS.is_eac (I.prefix itsl i) /\
+                   not (SpecTS.is_eac (I.prefix itsl (i + 1)))))
+        (ensures (SpecTS.eac_boundary itsl = i)) 
+        [SMTPat (I.prefix itsl i)]
+        = admit()
+
+let inductive_step_get #vcfg 
+                       (ils: IntTS.hash_verifiable_log vcfg) 
+                       (i:I.seq_index ils{let ils_i = I.prefix ils i in
+                                              induction_props ils_i /\
+                                              IntL.Get_S? (I.index ils i)}): induction_props_or_hash_collision (I.prefix ils (i + 1)) = 
+  let ilk = to_logk ils in  
+  let ils_i = I.prefix ils i in
+  let ilk_i = I.prefix ilk i in
+  let ils_i1 = I.prefix ils (i + 1) in
+  let ilk_i1 = I.prefix ilk (i + 1) in  
+
+  let vss_i = thread_state_pre ils i in
+  let vsk_i = SpecTS.thread_state_pre ilk i in 
+  let es = I.index ils i in
+  SpecTS.lemma_verifier_thread_state_extend ilk i;
+  
+  match es with
+  
+  | Get_S s k v ->
+    lemma_vget_simulates_spec vss_i vsk_i es;
+    lemma_forall_vtls_rel_extend ils i;    
+    lemma_vget_preserves_ismap vss_i es;
+    lemma_forall_store_ismap_extend ils i;
+    
+    if SpecTS.is_eac ilk_i1 then
+      None    
+    else (
+      lemma_eac_boundary_inv ilk_i1 i;
+      Some (lemma_non_eac_get_implies_hash_collision ilk_i1)
+    )
+
+let inductive_step_put #vcfg 
+                       (ils: IntTS.hash_verifiable_log vcfg) 
+                       (i:I.seq_index ils{let ils_i = I.prefix ils i in
+                                              induction_props ils_i /\
+                                              IntL.Put_S? (I.index ils i)}): induction_props_or_hash_collision (I.prefix ils (i + 1)) = 
+  let ilk = to_logk ils in  
+  let ils_i = I.prefix ils i in
+  let ilk_i = I.prefix ilk i in
+  let ils_i1 = I.prefix ils (i + 1) in
+  let ilk_i1 = I.prefix ilk (i + 1) in  
+
+  let vss_i = thread_state_pre ils i in
+  let vsk_i = SpecTS.thread_state_pre ilk i in 
+  let es = I.index ils i in
+  SpecTS.lemma_verifier_thread_state_extend ilk i;
+  
+  match es with
+  
+  | Put_S s k v -> 
+    lemma_vput_simulates_spec vss_i vsk_i es;
+    lemma_forall_vtls_rel_extend ils i;        
+    lemma_vput_preserves_ismap vss_i es;
+    lemma_forall_store_ismap_extend ils i;
+    if SpecTS.is_eac ilk_i1 then
+      None    
+    else (
+      lemma_eac_boundary_inv ilk_i1 i;
+      Some (lemma_non_eac_put_implies_hash_collision ilk_i1)
+    )  
+
 (* 
  * induction step: if all the induction properties hold for prefix of length i, 
  * then the properties hold for prefix of length (i + 1) or we construct 
@@ -45,7 +119,8 @@ let inductive_step #vcfg
                                       induction_props ils_i}): induction_props_or_hash_collision (I.prefix ils (i + 1)) = 
   let es = I.index ils i in 
   match es with
-  | IntL.Get_S _ _ _ -> admit()
+  | IntL.Get_S _ _ _ -> inductive_step_get ils i
+  | IntL.Put_S _ _ _ -> inductive_step_put ils i  
   | _ -> admit()                                      
 
 let lemma_empty_implies_induction_props #vcfg (ils: its_log vcfg{I.length ils = 0})
